cfi/refinementSC.v
@@ -1,0 +1,304 @@
+Require Import Coq.Lists.List.
+Require Import lib.utils.
+Require Import lib.partial_maps.
+Require Import lib.Coqlib.
+Require Import common.common.
+Require Import symbolic.symbolic.
+Require Import concrete.concrete.
+Require Import cfi.concrete.
+Require Import cfi.symbolic.
+Require Import cfi.preservation.
+Require Import cfi.rules.
+Require Import cfi.refinementAS. (*for Map - should remove when we move it*)
+
+Require Import ssreflect ssrfun ssrbool eqtype ssrnat seq.
+
+Set Implicit Arguments.
+
+
+Module MapTP.
+  Import TotalMaps.
+  Import PartMaps.
+
+Section Mappable.
+  Variable M1 M2 K V1 V2 : Type.
+
+  
+  Class mappable (tm1 : total_map M1 K V1) (pm2 : partial_map M2 K V2) := {
+
+    map : (V1 -> option V2) -> M1 -> M2;
+
+    map_correctness: forall (f : V1 -> option V2) (m1 : M1) (k : K),
+                       PartMaps.get (map f m1) k = f (TotalMaps.get m1 k)
+
+
+    }.
+End Mappable. 
+
+End MapTP.
+
+Import PartMaps.
+
+Section Refinement.
+
+
+Context {mt : machine_types}
+        {ops : machine_ops mt}
+        {opss : machine_ops_spec ops}
+
+        {cp : Concrete.concrete_params mt}
+        {sp : Concrete.params_spec cp}
+        {e : @rules.encodable (@rules.cfi_tag_eqType mt) mt ops}
+
+        {smemory : Type}
+        {sm : partial_map smemory (word mt) (atom (word mt) (@cfi_tag mt))}
+        {smems : axioms sm}
+
+        {sregisters : Type}
+        {sr : partial_map sregisters (reg mt) (atom (word mt) (@cfi_tag mt))}
+        {sregs : axioms sr}
+
+        {cm_map : Map.mappable (@Concrete.mem_class mt cp) sm}
+        {cr_map : MapTP.mappable (@Concrete.reg_class mt cp) sr}.
+
+Variable valid_jmp : word mt -> word mt -> bool.
+
+Definition sym_params := Sym.sym_cfi valid_jmp.
+
+Variable stable : list (@Symbolic.syscall mt sym_params).
+
+Variable ki : (@refinement_common.kernel_invariant mt ops sym_params cp e).
+
+Definition masks := symbolic.rules.masks.
+
+Definition refine_user_state (sst : Symbolic.state mt) (cst : Concrete.state mt) :=
+  refinement_common.refine_state ki stable sst cst.
+
+Definition refine_kernel_state (st : Symbolic.state mt) (kst : Concrete.state mt) :=
+  refinement_common.in_kernel kst = true /\
+  exists (ust : Concrete.state mt), 
+    (@refinement_common.in_user mt ops sym_params cp e) ust = true /\
+    exists kst', Concrete.step _ masks ust kst' /\ 
+                restricted_exec (fun s s' => Concrete.step _ masks s s') 
+                                (fun s => refinement_common.in_kernel s = true) 
+                                kst' kst /\
+                refine_user_state st ust.
+
+Definition refine_state (sst : Symbolic.state mt) (cst : Concrete.state mt) :=
+  refine_user_state sst cst \/ refine_kernel_state sst cst.
+
+Definition is_user (x : atom (word mt) (word mt)) := 
+  rules.word_lift (fun t => rules.is_user t) (common.tag x).
+
+Definition coerce (x : atom (word mt) (word mt)) : atom (word mt) (@cfi_tag mt) := 
+  match rules.decode (common.tag x) with
+    | Some (rules.USER tg) => (common.val x)@tg
+    | _ => (common.val x)@DATA (*this is unreachable in our case, dummy value*)
+  end.
+
+(*Q: Why can't I get it to typecheck when I substitute the existential with what
+  I use to instantiate it?*)
+Lemma mem_refinement_equiv :
+  forall (smem : @Symbolic.memory mt sym_params) cmem cmem',
+    refinement_common.refine_memory smem cmem ->
+    Conc.equiv cmem cmem' ->
+    exists (smem' : @Symbolic.memory mt sym_params),
+    refinement_common.refine_memory smem' cmem' /\
+    Sym.equiv smem smem'.
+Proof.
+  intros smem cmem cmem' REF EQUIV.
+  exists (Map.map coerce (filter is_user cmem')).
+  split.
+  { (*refinement proof*)
+    intros addr v tg.
+    split.
+    { intro CGET.
+      rewrite Map.map_correctness. rewrite filter_correctness.
+      rewrite CGET. simpl. 
+      destruct (is_user v@(rules.encode (rules.USER (user_tag:=cfi_tag_eqType) tg))) eqn:USER.
+      + simpl. unfold coerce. simpl. rewrite rules.decodeK. reflexivity.
+      + unfold is_user in USER. simpl in USER.
+        unfold rules.word_lift in USER.
+        rewrite rules.decodeK in USER. simpl in USER. discriminate. }
+    { intro SGET.
+      rewrite Map.map_correctness filter_correctness in SGET.
+      destruct (get cmem' addr) eqn:CGET.
+      - destruct a as [cv ctg].
+        simpl in SGET.
+        unfold is_user, rules.word_lift in SGET.
+        destruct (rules.decode ctg) eqn:CTG.
+        + destruct t; rewrite CTG in SGET; simpl in *.
+          * unfold coerce in SGET. rewrite CTG in SGET.
+            simpl in SGET. inv SGET.
+            simpl. apply rules.encodeK in CTG. rewrite CTG. reflexivity.
+          * discriminate.
+          * discriminate.
+        + rewrite CTG in SGET. simpl in SGET; discriminate.
+      - simpl in SGET. discriminate.
+    }
+  }
+  { (*equiv proof*)
+    unfold Sym.equiv, pointwise.
+    intro addr.
+    unfold Conc.equiv in EQUIV. unfold pointwise in EQUIV.
+    specialize (EQUIV addr).
+    destruct (get smem addr) eqn:SGET.
+    - destruct a as [v utg].
+      unfold refinement_common.refine_memory in REF.
+      specialize (REF addr v utg).
+      destruct REF as [REFCS REFSC].
+      assert (CGET := REFSC SGET).
+      rewrite CGET in EQUIV.
+      destruct (get cmem' addr) eqn:CGET'.
+      + destruct a as [v' ctg'].
+        inversion EQUIV 
+          as [a a' v0 v'' ut ut' EQ1 EQ2 SEQUIV| a a' ut ut' CONTRA ? ? |a a' CONTRA]; subst.
+        * rewrite Map.map_correctness filter_correctness.
+          rewrite CGET'.
+          unfold is_user. unfold rules.word_lift.
+          simpl. inversion EQ1; inversion EQ2; subst.
+          rewrite rules.decodeK.
+          simpl. unfold coerce.
+          simpl. rewrite rules.decodeK.
+          apply rules.encode_inj in H1.
+          inversion H1; subst.
+          assumption.
+        * apply rules.encode_inj in CONTRA.
+          inversion CONTRA.
+        * simpl in CONTRA. apply rules.encode_inj in CONTRA.
+          inversion CONTRA.
+      + destruct EQUIV.
+    - destruct (get cmem addr) eqn:CGET.
+      + destruct a as [v ctg]. unfold refinement_common.refine_memory in REF.
+        rewrite Map.map_correctness filter_correctness.
+        unfold is_user. unfold rules.word_lift.
+        destruct (get cmem' addr) eqn:CGET'.
+        * destruct a as [v' ctg'].
+          simpl.
+          destruct (rules.decode ctg') eqn:DECODE.
+          - destruct (rules.is_user t) eqn:USER.
+            + simpl.
+              unfold rules.is_user in USER.
+              destruct t; try discriminate.
+              apply rules.encodeK in DECODE.
+              rewrite <- DECODE in EQUIV.
+               inversion EQUIV 
+          as [a a' v0 v'' ? ? EQ1 EQ2 SEQUIV| a a' ? ? ? CONTRA ? |a a' ? CONTRA];
+                subst.
+               { inversion EQ1; subst.
+                 apply REF in CGET. rewrite SGET in CGET; discriminate. }
+               { simpl in CONTRA. apply rules.encode_inj in CONTRA.
+                 inversion CONTRA. }
+               { simpl in CONTRA. apply rules.encode_inj in CONTRA.
+                 inversion CONTRA. }
+            + simpl. constructor.
+          - simpl. constructor.
+        * destruct EQUIV.
+     + destruct (get cmem' addr) eqn:CGET'.
+       * destruct EQUIV.
+       * rewrite Map.map_correctness filter_correctness.
+         rewrite CGET'. simpl. constructor.
+  }
+Qed.
+    
+Definition creg_to_sreg x :=
+  match is_user x with
+    | true => Some (coerce x)
+    | false => None
+  end.
+
+Lemma reg_refinement_equiv :
+  forall (sregs : @Symbolic.registers mt sym_params) cregs cregs',
+    refinement_common.refine_registers sregs cregs ->
+    Conc.reg_equiv cregs cregs' ->
+    exists (sregs' : @Symbolic.registers mt sym_params),
+    refinement_common.refine_registers sregs' cregs' /\
+    Sym.equiv sregs sregs'.
+Proof.
+  intros sreg creg creg' REF EQUIV.
+  exists (MapTP.map creg_to_sreg creg').
+  split.
+  { (*Refinement proof*)
+    intros n v tg.
+    split.
+    { intros CGET'.
+      rewrite MapTP.map_correctness. 
+      rewrite CGET'. simpl. 
+      unfold creg_to_sreg.
+      destruct (is_user v@(rules.encode (rules.USER (user_tag:=cfi_tag_eqType) tg))) eqn:USER.
+      + simpl. unfold coerce. simpl. rewrite rules.decodeK. reflexivity.
+      + unfold is_user in USER. simpl in USER.
+        unfold rules.word_lift in USER.
+        rewrite rules.decodeK in USER. simpl in USER. discriminate. }
+    { intro SGET'.
+      rewrite MapTP.map_correctness in SGET'.
+      destruct (TotalMaps.get creg' n) eqn:CGET'.
+      simpl in SGET'.
+      unfold creg_to_sreg in SGET'.
+      unfold is_user, rules.word_lift in SGET'.
+      simpl in SGET'.
+      destruct (rules.decode tag) eqn:CTG.
+      + unfold rules.is_user, coerce in SGET'. destruct t; simpl in CTG.
+        * rewrite CTG in SGET'.
+          simpl in SGET'. inv SGET'.
+          simpl. apply rules.encodeK in CTG. rewrite CTG. reflexivity.
+        * discriminate.
+        * discriminate.
+      + discriminate. 
+    }
+  }
+  { (*equiv proof*)
+    unfold Sym.equiv, pointwise.
+    intro n.
+    unfold Conc.reg_equiv in EQUIV.
+    specialize (EQUIV n).
+    destruct (get sreg n) eqn:SGET.
+    - destruct a as [v utg].
+      specialize (REF n v utg).
+      destruct REF as [REFCS REFSC].
+      assert (CGET := REFSC SGET).
+      rewrite CGET in EQUIV.
+      rewrite MapTP.map_correctness. 
+      destruct (TotalMaps.get creg' n) eqn:CGET'.
+      inversion EQUIV 
+        as [a a' v0 v'' ut ut' EQ1 EQ2 SEQUIV| a a' ut ut' CONTRA ? ? |a a' CONTRA]; subst.
+      * inv EQ2.
+        unfold creg_to_sreg, is_user, rules.word_lift, coerce, rules.is_user.
+        simpl. rewrite rules.decodeK.
+        inv EQ1.
+        apply rules.encode_inj in H1. inv H1.
+        assumption.
+      * apply rules.encode_inj in CONTRA.
+          inversion CONTRA.
+      * simpl in CONTRA. apply rules.encode_inj in CONTRA.
+          inversion CONTRA.
+    - rewrite MapTP.map_correctness.
+      destruct (TotalMaps.get creg' n) eqn:CGET'.
+      destruct (TotalMaps.get creg n) eqn:CGET.
+      inversion EQUIV 
+        as [a a' v0 v'' ? ? EQ1 EQ2 SEQUIV| a a' ? ? EQ1 EQ2 EQ3 |a a' EQ1 EQ2 EQ3];
+        subst.
+       + inv EQ1.
+         apply REF in CGET.
+         rewrite CGET in SGET. discriminate.
+       + inv EQ3.
+         unfold creg_to_sreg, is_user, rules.word_lift, coerce.
+         rewrite EQ1. rewrite rules.decodeK. simpl.
+         constructor.
+       + inv EQ3.
+         unfold creg_to_sreg, is_user, rules.word_lift, coerce.
+         rewrite EQ1. rewrite rules.decodeK. simpl.
+         constructor.
+  }
+Qed.  
+
+Theorem backwards_simulation_attacker sst cst cst' :
+  refine_state sst cst ->
+  Conc.step_a valid_jmp cst cst' ->
+  exists sst',
+    Sym.step_a stable sst sst' /\
+    refine_state sst' cst'.
+Proof. 
+  intros REF STEP.
+  inversion STEP; subst.
+  unfold Conc.equiv in MEQUIV. unfold pointwise in MEQUIV.
